src/Rupicola/Lib/Api.v
@@ -1,4 +1,5 @@
 Require Export Rupicola.Lib.Core.
+Require Export Rupicola.Lib.Monads.
 Require Export Rupicola.Lib.Tactics.
 Require Export Rupicola.Lib.Notations.
 Require Export Rupicola.Lib.Compiler.
